proof/security/MLWE_PKE.ec
@@ -1,5 +1,5 @@
-require import AllCore Distr List SmtMap Dexcepted.
-require (****) RndExcept StdOrder PKE_Ext MLWE.
+require import AllCore Distr List SmtMap Dexcepted PKE_ROM.
+require (****) RndExcept StdOrder MLWE.
 
 theory MLWE_PKE.
 
@@ -37,7 +37,7 @@ axiom sk_encodeK : cancel sk_encode sk_decode.
 (******************************************************************)
 (*    The Security Games                                          *)
 
-clone import PKE_Ext as PKE_ with 
+clone import PKE_ROM with 
   type RO.in_t    = RO_SMP.in_t,
   type RO.out_t   = RO_SMP.out_t,  
   op   RO.dout    = RO_SMP.dout,  
@@ -57,7 +57,8 @@ import RO_SMP.
    This PKE does not use the RO directly but may
    do so via the Sampler *)
 
-module MLWE_PKE(S: PSampler, O : ROpub) : Scheme = {
+
+module MLWE_PKE(S: PSampler, O : POracle) (* : Scheme *) = {
   proc kg() : pkey * skey = {
     var sd,s,e,_A,t;
     sd <$ dseed;
@@ -87,222 +88,6 @@ module MLWE_PKE(S: PSampler, O : ROpub) : Scheme = {
   }
 }.
 
-(******************************************************************)
-(*       Game Hopping Security for Concrete Hash                  *)
-(******************************************************************)
-
-module HS : PSampler = { 
-      proc sampleA(sd : seed) = { return H sd; } 
-      proc sampleAT(sd : seed) = { return trmx (H sd); } }.
-module NULL : ROpub = 
-   { proc h(x : in_t) : out_t = { return witness; }  }.
-module MLWE_PKE_H = MLWE_PKE(HS,NULL).
-
-(* Hop 1 *)
-
-module MLWE_PKE1(S : PSampler, O : ROpub) = {
-  proc kg() : pkey * skey = {
-    var _A,sd,s,t;
-    sd <$ dseed;
-    s  <$ dshort;
-    t  <$ duni;
-    _A <@ S.sampleA(sd);
-    return (pk_encode (t,sd),sk_encode s);
-  }
-
-  include MLWE_PKE(S,NULL) [-kg]
-
-}.
-
-module B1(A : Adversary) : HAdv_T = {
-
-  proc kg(t : vector, sd : seed) : pkey * skey = {
-    return (pk_encode (t,sd),witness);
-  }
-  
-  proc guess(sd : seed, t : vector, uv : vector * R) : bool = {
-    var pk, sk, m0, m1, c, b, b';
-    (pk,sk) <@ kg(uv.`1,sd);
-    (m0, m1) <@ A.choose(pk);
-    b <$ {0,1};
-    c <@ MLWE_PKE_H.enc(pk, if b then m1 else m0);
-    b' <@ A.guess(c);
-    return b' = b;
-  }
-}.
-
-section.
-
-declare module A <: Adversary.
-
-lemma hop1_left &m: 
-  Pr[CPA(MLWE_PKE_H,A).main() @ &m : res] =
-  Pr[MLWE_H(B1(A)).main(false,false) @ &m : res].
-proof.
-byequiv => //. 
-proc; inline *. 
-wp; call(:true); auto => /=. 
-call (:true); wp.
-by rnd{2}; wp; do 3! rnd{2}; auto; smt(duni_ll).
-qed.
-
-lemma hop1_right &m: 
-  Pr[MLWE_H(B1(A)).main(false,true) @ &m : res] = 
-  Pr[CPA(MLWE_PKE1(HS,NULL),A).main() @ &m : res].
-proof.
-byequiv => //.
-proc;inline *. 
-wp; call(:true); auto => /=.
-call(:true); wp => /=.
-rnd{1}; wp; do 2! rnd{1}.
-by rnd; wp; rnd{1}; auto; smt(duni_ll dshort_ll).
-qed.
-
-end section.
-
-(* Hop 2 *)
-
-module MLWE_PKE2(S : PSampler, O : ROpub) = {
-
-  proc enc(pk : pkey, m : plaintext) : ciphertext = {
-    var _A,u, v;
-    _A <@ S.sampleAT((pk_decode pk).`2);
-    u <$duni;
-    v <$duni_R;
-    return (c_encode (u,v &+ m_encode m));
-  }
-
-  include MLWE_PKE1(S,O) [-enc]
-
-}.
-
-module B2(A : Adversary) : HAdv_T = {
-
-  proc kg(t : vector, sd : seed) : pkey * skey = {
-    return (pk_encode (t,sd),witness);
-  }
-  
-  proc enc(pk : pkey, m : plaintext, uv : vector * R) : ciphertext = {
-    return (c_encode (uv.`1, uv.`2 &+ m_encode m));
-  }
-  
-  proc guess(sd : seed, t : vector, uv : vector * R) : bool = {
-    var pk, sk, m0, m1, c, b, b';
-    (pk,sk) <@ kg(t,sd);
-    (m0, m1) <@ A.choose(pk);
-    b <$ {0,1};
-    c <@ enc(pk, if b then m1 else m0,uv);
-    b' <@ A.guess(c);
-    return b' = b;
-  }
-
-}.
-
-section.
-
-declare module A <: Adversary.
-
-lemma hop2_left &m: 
-  Pr[CPA(MLWE_PKE1(HS,NULL),A).main() @ &m : res] =
-  Pr[MLWE_H(B2(A)).main(true,false) @ &m : res].
-proof.
-byequiv => //.
-proc; inline *. 
-swap {2} 7 -5.
-swap {2} [11..12] -8.
-swap {2} [14..17] -9.
-seq 6 7 : (#pre /\ ={sd,t,pk} /\ (pk_decode pk{2}).`2 = sd{2} /\ (pk_decode pk{2}).`1 = t{2});
-  first by wp;rnd; rnd{1}; rnd; auto; smt(dshort_ll pk_encodeK).
-swap {2} [11..13] -9.
-by wp; call(_: true); wp; rnd{2}; wp; rnd; rnd{2}; wp; 
-   rnd; rnd; wp; rnd; call(_: true); auto; smt(duni_ll dshort_ll).
-qed.
-
-lemma hop2_right &m: 
-  Pr[MLWE_H(B2(A)).main(true,true) @ &m : res] = 
-  Pr[CPA(MLWE_PKE2(HS,NULL),A).main() @ &m : res].
-proof.
-byequiv => //.
-proc; inline *. 
-swap {1} 7 -5.
-swap {1} [11..12] -8.
-swap {1} [14..17] -9.
-seq 7 6 : (#pre /\ ={sd,t,pk} /\ (pk_decode pk{2}).`2 = sd{2} /\ (pk_decode pk{2}).`1 = t{2});
-   first by wp;rnd;  rnd{2}; rnd; auto; smt(dshort_ll pk_encodeK). 
-swap {1} [11..13] -9.
-by wp; call(_: true);wp;rnd;wp;rnd{1};rnd;wp;rnd{1};rnd{1};wp;rnd; 
-   call(_: true); auto;smt(duni_ll dshort_ll).
-qed.
-
-end section.
-
-(* Final game analysis *)
-
-section.
-
-declare module A <: Adversary.
-
-local module Game2(A : Adversary) = {
-  proc main() = {
-    var sd, s, t, m0, m1, u, v, b, b';
-    sd <$ dseed;
-    s <$ dshort;
-    t <$ duni;
-    (m0, m1) <@ A.choose(pk_encode (t,sd));
-    u <$duni;
-    v <$duni_R;
-    b' <@ A.guess(c_encode (u,v));
-    b <$ {0,1};
-    return b = b';
-  }
-}.
-
-local lemma game2_equiv &m :
-  Pr[CPA(MLWE_PKE2(HS,NULL),A).main() @ &m : res] = 
-  Pr[Game2(A).main() @ &m : res].
-proof.
-byequiv => //.
-proc; inline *.
-swap {2} 8 -3.
-call(_: true); wp.
-rnd (fun z, z &+ m_encode (if b then m1 else m0){2})
-    (fun z, z &- m_encode (if b then m1 else m0){2}).
-auto; call (_:true).
-auto => /> *; split => *; [ ring | split => *; [ring | smt()]].
-qed.
-
-local lemma game2_prob &m :
-  islossless A.guess => islossless A.choose =>
-  Pr[Game2(A).main() @ &m : res] = 1%r / 2%r.
-proof.
-move => A_guess_ll A_choose_ll.
-byphoare => //. 
-proc.
-rnd  (pred1 b')=> //=.
-conseq (: _ ==> true).
-+ by move=> />; apply DBool.dbool1E.
-by islossless; smt(duni_ll dshort_ll). 
-qed.
-
-lemma main_theorem &m :
-  islossless A.guess => islossless A.choose =>
-  Pr[CPA(MLWE_PKE_H,A).main() @ &m : res] -  1%r / 2%r =
-    Pr[MLWE_H(B1(A)).main(false,false) @ &m : res] -
-       Pr[MLWE_H(B1(A)).main(false,true) @ &m : res] + 
-    Pr[MLWE_H(B2(A)).main(true,false) @ &m : res] -
-       Pr[MLWE_H(B2(A)).main(true,true) @ &m : res].
-proof.
-move => A_guess_ll A_choose_ll.
-rewrite (hop1_left A &m).
-rewrite (hop1_right A &m).
-rewrite (hop2_left A &m).
-rewrite (hop2_right A &m).
-rewrite (game2_equiv &m).
-rewrite (game2_prob &m _ _) //.
-by ring.
-qed.
-
-end section.
 
 (******************************************************************)
 (*       Game Hopping Security for Sampler                        *)
@@ -313,7 +98,22 @@ module MLWE_PKE_RO(S : PSampler) = MLWE_PKE(S).
 
 (* Hop 1 *)
 
-module (B1ROM(A : AdversaryRO, S : Sampler) : SAdv_T) (H : ROpub) = {
+module MLWE_PKE1(S : PSampler, O : POracle) = {
+  proc kg() : pkey * skey = {
+    var _A,sd,s,t;
+    sd <$ dseed;
+    s  <$ dshort;
+    t  <$ duni;
+    _A <@ S.sampleA(sd);
+    return (pk_encode (t,sd),sk_encode s);
+  }
+
+  include MLWE_PKE(S,O) [-kg]
+
+}.
+
+
+module (B1ROM(A : Adversary, S : Sampler) : SAdv_T) (H : POracle) = {
   var sd : seed
   var t  : vector
   
@@ -334,10 +134,10 @@ section.
 
 declare module O <: RO {-B1ROM}.
 declare module S <: Sampler {-O,-B1ROM}.
-declare module A <: AdversaryRO {-O,-B1ROM,-S}.
+declare module A <: Adversary {-O,-B1ROM,-S}.
 
 lemma hop1_left_s &m: 
-  Pr[CPAROM(MLWE_PKE(S(Pub(O))),A,O).main() @ &m : res] =
+  Pr[CPA(O,MLWE_PKE(S(O)),A).main() @ &m : res] =
   Pr[MLWE_SMP(B1ROM(A,S),S,O).main(false,false) @ &m : res].
 proof.
 byequiv => //.
@@ -356,7 +156,7 @@ by wp;rnd{2};rnd;rnd;rnd;auto => />;smt(dshort_ll duni_ll).
 qed.
 
 lemma hop1_right_s &m: 
-  Pr[CPAROM(MLWE_PKE1(S(Pub(O))),A,O).main() @ &m : res] =
+  Pr[CPA(O,MLWE_PKE1(S(O)),A).main() @ &m : res] =
   Pr[MLWE_SMP(B1ROM(A,S),S,O).main(false,true) @ &m : res].
 proof.
 byequiv => //.
@@ -377,7 +177,24 @@ qed.
 
 end section.
 
-module (B2ROM(A : AdversaryRO, S : Sampler) : SAdv_T) (H : ROpub) = {
+(* Hop 2 *)
+
+module MLWE_PKE2(S : PSampler, O : POracle) = {
+
+  proc enc(pk : pkey, m : plaintext) : ciphertext = {
+    var _A,u, v;
+    _A <@ S.sampleAT((pk_decode pk).`2);
+    u <$duni;
+    v <$duni_R;
+    return (c_encode (u,v &+ m_encode m));
+  }
+
+  include MLWE_PKE1(S,O) [-enc]
+
+}.
+
+
+module (B2ROM(A : Adversary, S : Sampler) : SAdv_T) (H : POracle) = {
   var pk : pkey
   var m0, m1 : plaintext
 
@@ -406,10 +223,10 @@ section.
 
 declare module O <: RO {-B2ROM}.
 declare module S <: Sampler {-O,-B2ROM}.
-declare module A <: AdversaryRO {-O,-B2ROM, -S}.
+declare module A <: Adversary {-O,-B2ROM, -S}.
 
 lemma hop2_left_s &m: 
-  Pr[CPAROM(MLWE_PKE1(S(Pub(O))),A,O).main() @ &m : res] =
+  Pr[CPA(O,MLWE_PKE1(S(O)),A).main() @ &m : res] =
   Pr[MLWE_SMP(B2ROM(A,S),S,O).main(true,false) @ &m : res].
 proof.
 byequiv => //.
@@ -429,7 +246,7 @@ by wp; rnd; wp; rnd; rnd{1}; auto => />; smt(dshort_ll duni_ll pk_encodeK).
 qed.
 
 lemma hop2_right_s &m: 
-  Pr[CPAROM(MLWE_PKE2(S(Pub(O))),A,O).main() @ &m : res] =
+  Pr[CPA(O,MLWE_PKE2(S(O)),A).main() @ &m : res] =
   Pr[MLWE_SMP(B2ROM(A,S),S,O).main(true,true) @ &m : res].
 proof.
 byequiv => //.
@@ -457,22 +274,21 @@ section.
 
 declare module O <: RO {-B1ROM, -B2ROM}.
 declare module S <: Sampler {-O, -B1ROM, -B2ROM}.
-declare module A <: AdversaryRO {-O, -B1ROM, -B2ROM, -S}.
+declare module A <: Adversary {-O, -B1ROM, -B2ROM, -S}.
 
-local module Game2RO(A : AdversaryRO) = {
-  module H = Pub(O)
+local module Game2RO(A : Adversary) = {
   proc main() = {
     var sd, _A, s, t, m0, m1, u, v, b, b';
     O.init();
     sd <$ dseed;
-    _A <@ S(H).sampleA(sd);
+    _A <@ S(O).sampleA(sd);
     s <$ dshort;
     t <$ duni;
-    (m0, m1) <@ A(H).choose(pk_encode (t,sd));
-    _A <@ S(H).sampleAT(sd);
+    (m0, m1) <@ A(O).choose(pk_encode (t,sd));
+    _A <@ S(O).sampleAT(sd);
     u <$duni;
     v <$duni_R;
-    b' <@ A(H).guess(c_encode (u,v));
+    b' <@ A(O).guess(c_encode (u,v));
     b <$ {0,1};
     return b = b';
   }
@@ -480,7 +296,7 @@ local module Game2RO(A : AdversaryRO) = {
 
 
 local lemma game2_equiv_s &m : 
-  Pr[CPAROM(MLWE_PKE2(S(Pub(O))),A,O).main() @ &m : res] = 
+  Pr[CPA(O,MLWE_PKE2(S(O)),A).main() @ &m : res] = 
   Pr[Game2RO(A).main() @ &m : res].
 proof.
 byequiv => //.
@@ -504,17 +320,17 @@ qed.
 local lemma game2_prob_s &m :
   islossless O.init =>
   islossless O.get =>
-  (forall (O <: ROpub), islossless O.h => islossless S(O).sampleA) =>   
-  (forall (O <: ROpub), islossless O.h => islossless S(O).sampleAT) =>   
-  (forall (O <: ROpub), islossless O.h => islossless A(O).guess) =>
-  (forall (O <: ROpub), islossless O.h => islossless A(O).choose) =>
+  (forall (O <: POracle), islossless O.get => islossless S(O).sampleA) =>   
+  (forall (O <: POracle), islossless O.get => islossless S(O).sampleAT) =>   
+  (forall (O <: POracle), islossless O.get => islossless A(O).guess) =>
+  (forall (O <: POracle), islossless O.get => islossless A(O).choose) =>
   Pr[Game2RO(A).main() @ &m : res] = 1%r / 2%r.
 proof.
 move => O_init_ll O__o_ll SA_ll SAT_ll A_guess_ll A_choose_ll.
-move : (SAT_ll (Pub(O))).
-move : (SA_ll (Pub(O))).
-move : (A_guess_ll (Pub(O))).
-move : (A_choose_ll (Pub(O))).
+move : (SAT_ll (O)).
+move : (SA_ll (O)).
+move : (A_guess_ll (O)).
+move : (A_choose_ll (O)).
 move => _A_choose_ll _A_guess_ll _SA_ll _SAT_ll.
 byphoare => //;proc.
 rnd  (pred1 b')=> //=; conseq (: _ ==> true).
@@ -529,11 +345,11 @@ qed.
 lemma main_theorem_s &m :
   islossless O.init =>
   islossless O.get =>
-  (forall (O <: ROpub), islossless O.h => islossless S(O).sampleA) =>   
-  (forall (O <: ROpub), islossless O.h => islossless S(O).sampleAT) =>   
-  (forall (O <: ROpub), islossless O.h => islossless A(O).guess) =>
-  (forall (O <: ROpub), islossless O.h => islossless A(O).choose) =>
-  Pr[CPAROM(MLWE_PKE(S(Pub(O))),A,O).main() @ &m : res] -  1%r / 2%r =
+  (forall (O <: POracle), islossless O.get => islossless S(O).sampleA) =>   
+  (forall (O <: POracle), islossless O.get => islossless S(O).sampleAT) =>   
+  (forall (O <: POracle), islossless O.get => islossless A(O).guess) =>
+  (forall (O <: POracle), islossless O.get => islossless A(O).choose) =>
+  Pr[CPA(O,MLWE_PKE(S(O)),A).main() @ &m : res] -  1%r / 2%r =
     Pr[MLWE_SMP(B1ROM(A,S),S,O).main(false,false) @ &m : res] -
        Pr[MLWE_SMP(B1ROM(A,S),S,O).main(false,true) @ &m : res] + 
     Pr[MLWE_SMP(B2ROM(A,S),S,O).main(true,false) @ &m : res] -
@@ -563,22 +379,22 @@ import MLWE_ROM.
 
 section. 
 
-declare module A <: AdversaryRO {-B1ROM, -B2ROM, -LRO, -RO_H.RO, -RO_H.FRO, -RO_H.LRO, -B,-Bt, -BS, -D}.
+declare module A <: Adversary {-B1ROM, -B2ROM, -LRO, -RO_H.RO, -RO_H.FRO, -RO_H.LRO, -B,-Bt, -BS, -D}.
 declare module S <: Sampler {-A, -B1ROM, -B2ROM, -LRO, -RO_H.RO, -RO_H.FRO, -RO_H.LRO, -B,-Bt, -BS, -D}.
 declare module Sim <: Simulator_t {-S,-A,-B1ROM, -B2ROM, -LRO, -RO_H.RO, -RO_H.FRO, -RO_H.LRO, -B,-Bt, -BS, -D}.
 
 lemma main_theorem_ref &m epsilon :
   0%r <= epsilon =>
   (forall (x : RO_SMP.in_t), is_lossless (RO_SMP.dout x)) => 
-  (forall (O <: RO_SMP.ROpub), islossless O.h => islossless S(O).sampleA) =>
-  (forall (O <: RO_SMP.ROpub), islossless O.h => islossless S(O).sampleAT) =>
-  (forall (O <: RO_SMP.ROpub), islossless O.h => islossless A(O).guess) =>
-  (forall (O <: RO_SMP.ROpub), islossless O.h => islossless A(O).choose) =>
+  (forall (O <: SMP_RO), islossless O.get => islossless S(O).sampleA) =>
+  (forall (O <: SMP_RO), islossless O.get => islossless S(O).sampleAT) =>
+  (forall (O <: SMP_RO), islossless O.get => islossless A(O).guess) =>
+  (forall (O <: SMP_RO), islossless O.get => islossless A(O).choose) =>
   (* We need indiff from the nice ROM *)
   (forall tr b (D0 <: Distinguisher_t {-S,-LRO, -RO, -RO_H.LRO, -RO_H.RO, -Sim}),
      `| Pr[ WIndfReal(D0,S,RO_SMP.LRO).main(tr,b) @ &m : res] - 
         Pr[ WIndfIdeal(D0,Sim,RO_H.LRO).main(tr,b) @ &m : res] | <= epsilon) =>
-  `| Pr[CPAROM(MLWE_PKE(S(RO_SMP.LROpub)),A,RO_SMP.LRO).main() @ &m : res] -  1%r / 2%r | <=
+  `| Pr[CPA(RO_SMP.LRO,MLWE_PKE(S(RO_SMP.LRO)),A).main() @ &m : res] -  1%r / 2%r | <=
     `| Pr[MLWE(B(BS(B1ROM(A,S),Sim),RO_H.LRO)).main(false) @ &m : res] -
        Pr[MLWE(B(BS(B1ROM(A,S),Sim),RO_H.LRO)).main(true) @ &m : res] | + 
     `| Pr[MLWE(Bt(BS(B2ROM(A,S),Sim),RO_H.LRO)).main(false) @ &m : res]-
@@ -672,20 +488,19 @@ axiom good_decode m n :
 
 (* We now rewrite the correctness game in terms of noise and move
    to the RO that directly samples a uniform matrix *)
-module CorrectnessAdvNoise(Sim : Simulator_t,A : CAdversaryRO, O : RO_H.RO) = {
-  module H = RO_H.Pub(O)
+module CorrectnessAdvNoise(Sim : Simulator_t,A : CORR_ADV, O : RO_H.RO) = {
   proc main() = {
     var sd,s,e,_A,r,e1,e2,m,n;
     O.init();
-    Sim(H).init();
+    Sim(O).init();
     sd <$ dseed;
-    _A <@ H.h(sd);
+    _A <@ O.get(sd);
     r <$ dshort;
     s <$ dshort;
     e <$ dshort;
     e1 <$ dshort;
     e2 <$ dshort_R;
-    m <@ A(Sim(H)).find(pk_encode (_A *^ s + e,sd),sk_encode s);
+    m <@ A(Sim(O)).find(pk_encode (_A *^ s + e,sd),sk_encode s);
     n <- noise_exp _A s e r e1 e2 m;
     return (!under_noise_bound n max_noise);
   }
@@ -693,11 +508,11 @@ module CorrectnessAdvNoise(Sim : Simulator_t,A : CAdversaryRO, O : RO_H.RO) = {
 
 section.
 
-declare module A <: CAdversaryRO {-LRO,-RO, -RO_H.RO, -RO_H.LRO}.
+declare module A <: CORR_ADV {-LRO,-RO, -RO_H.RO, -RO_H.LRO}.
 declare module S <: Sampler {-A,-LRO,-RO, -RO_H.RO, -RO_H.LRO}.
 declare module Sim <: Simulator_t {-S, -A,-LRO,-RO, -RO_H.RO, -RO_H.LRO}.
 
-module (D(A : CAdversaryRO) : Distinguisher_t) (S : PSampler, H : RO_SMP.ROpub) = {
+module (D(A : CORR_ADV) : Distinguisher_t) (S : PSampler, H : SMP_RO) = {
    proc distinguish(tr b : bool, sd : seed) : bool = {
      var t,r,e1,e2,u,v,c,u0,v0,m',b',s,e,_A, pk, sk, m;
      s <$ dshort;                                     
@@ -716,82 +531,77 @@ module (D(A : CAdversaryRO) : Distinguisher_t) (S : PSampler, H : RO_SMP.ROpub) 
      c <- c_encode (u, v);                              
      (u0, v0) <- c_decode c;                           
      m' <- Some (m_decode (v0 &- (sk_decode sk `<*>` u0)));
-     b' <- m' = Some m;                        
+     b' <- m' <> Some m;                        
      return b';
    }
 }.
 
 lemma correctness &m epsilon:
-  (forall (O <: RO_H.ROpub), islossless O.h => islossless Sim(O).init) =>
-  (forall (O <: RO_H.ROpub), islossless O.h => islossless Sim(O).h) =>
-  (forall (O <: RO_SMP.ROpub), islossless O.h => islossless A(O).find) =>
+  (forall (O <: Ideal_RO), islossless O.get => islossless Sim(O).init) =>
+  (forall (O <: Ideal_RO), islossless O.get => islossless Sim(O).get) =>
+  (forall (O <: SMP_RO), islossless O.get => islossless A(O).find) =>
   (* We need indiff from the nice ROM *)
   (forall trb (D0 <: Distinguisher_t {-S,-LRO, -RO, -RO_H.LRO,-RO_H.RO, -Sim}),
      `| Pr[ WIndfReal(D0,S,RO_SMP.LRO).main(trb) @ &m : res] - 
         Pr[ WIndfIdeal(D0,Sim,RO_H.LRO).main(trb) @ &m : res] | <= epsilon) =>
-  Pr[ CorrectnessAdvROM(MLWE_PKE(S(RO_SMP.LROpub)),A,RO_SMP.LRO).main() @ &m : res]  >=
-  1%r - Pr[ CorrectnessAdvNoise(Sim,A,RO_H.LRO).main() @ &m : res] - epsilon.
+  Pr[ Correctness_Adv(RO_SMP.LRO,MLWE_PKE(S(RO_SMP.LRO)),A).main() @ &m : res]  <= epsilon
+       + Pr[ CorrectnessAdvNoise(Sim,A,RO_H.LRO).main() @ &m : res].
 proof.
 move => Sim_init_ll Sim_h_ll A_ll HIND.
-have -> : 1%r - Pr[ CorrectnessAdvNoise(Sim,A,RO_H.LRO).main() @ &m : res] =
-   Pr[ CorrectnessAdvNoise(Sim,A,RO_H.LRO).main() @ &m : !res].
-rewrite Pr[mu_not]; congr => //. 
-+ byphoare => //.
-  islossless; 2..6: smt(duni_matrix_ll dshort_ll). 
-  + by apply (A_ll (Sim(RO_H.LROpub))); apply (Sim_h_ll (RO_H.LROpub)); apply RO_H.RO_get_ll; smt(duni_matrix_ll). 
-  by apply (Sim_init_ll (RO_H.LROpub));apply RO_H.RO_get_ll; smt(duni_matrix_ll). 
-have -> : Pr[CorrectnessAdvROM(MLWE_PKE(S(RO_SMP.LROpub)), A, RO_SMP.LRO).main() @ &m : res] = 
+have -> : Pr[Correctness_Adv(RO_SMP.LRO,MLWE_PKE(S(RO_SMP.LRO)), A).main() @ &m : res] = 
           Pr[ WIndfReal(D(A),S,RO_SMP.LRO).main(witness) @ &m : res].
-+ byequiv => //; proc. inline {1} 2. inline {1} 5. inline {1} 4. inline {1} 2. inline {2} 3. 
++ byequiv => //; proc;inline *; wp 22 21; conseq (:_ ==> ={m,m'}); 1: by smt(). 
   by sim. 
 have  := (HIND witness (D(A))).
 
-have ? : Pr[CorrectnessAdvNoise(Sim, A, RO_H.LRO).main() @ &m : !res] <=
-          Pr[WIndfIdeal(D(A), Sim, RO_H.LRO).main(witness) @ &m : res]; last by smt().
+have ? : 
+          Pr[WIndfIdeal(D(A), Sim, RO_H.LRO).main(witness) @ &m : res] <= 
+             Pr[CorrectnessAdvNoise(Sim, A, RO_H.LRO).main() @ &m : res]; last by smt().
 
 byequiv => //.
 proc.  
-inline {2} 4. 
-swap {2} 6 -2.
-swap {2} 9 -4.
-swap {2} [14..16] -8.
-swap {2} [11..12] -4.
-seq 10 15 : ( 
+inline {1} 4. 
+swap {1} 6 -2.
+swap {1} 9 -4.
+swap {1} [14..16] -8.
+swap {1} [11..12] -4.
+seq 15 10 : ( 
            ={RO_H.RO.m,e2,e1,r,s,e,sd,m,glob Sim} /\
-           sd0{2} = sd{2} /\
-           (pk_decode pk{2}).`2 = sd{2} /\
-           (pk_decode pk{2}).`1 = t{2} /\
-           sk_decode sk{2} = s{2} /\
-           t{2} = _A{2} *^ s{2} + e{2} /\
-           (pk_decode pk{2}).`2 \in RO_H.RO.m{2} /\
-           _A{2} = _A{1} /\
-           oget RO_H.RO.m{2}.[(pk_decode pk{2}).`2] = _A{2}); last first.
-+ inline *; auto => />; move => &2  ->?; split; 1: by smt(duni_matrix_ll). 
-  move => *;rewrite  encode_noise.
+           sd0{1} = sd{1} /\
+           (pk_decode pk{1}).`2 = sd{1} /\
+           (pk_decode pk{1}).`1 = t{1} /\
+           sk_decode sk{1} = s{1} /\
+           t{1} = _A{1} *^ s{1} + e{1} /\
+           (pk_decode pk{1}).`2 \in RO_H.RO.m{1} /\
+           _A{1} = _A{2} /\
+           oget RO_H.RO.m{1}.[(pk_decode pk{1}).`2] = _A{1}); last first.
++ inline *; auto => />; move => &1 &2  ->?; split; 1: by smt(duni_matrix_ll). 
+  move => ???;rewrite  encode_noise.
   rewrite (_: 
-     (((oget RO_H.RO.m{2}.[(pk_decode pk{2}).`2] *^ (sk_decode sk){2} + e{2}) `<*>` r{2}) &+
+     (((oget RO_H.RO.m{2}.[(pk_decode pk{1}).`2] *^ (sk_decode sk){1} + e{2}) `<*>` r{2}) &+
      e2{2} &+ m_encode m{2} &+
      rnd_err_v
-       (((oget RO_H.RO.m{2}.[(pk_decode pk{2}).`2] *^ (sk_decode sk){2}  + e{2}) `<*>` r{2}) &+
+       (((oget RO_H.RO.m{2}.[(pk_decode pk{1}).`2] *^ (sk_decode sk){1}  + e{2}) `<*>` r{2}) &+
         e2{2} &+ m_encode m{2}) &-
-     ((sk_decode sk){2}  `<*>`
-      (m_transpose (oget RO_H.RO.m{2}.[(pk_decode pk{2}).`2]) *^ r{2} + e1{2} +
-       rnd_err_u (m_transpose (oget RO_H.RO.m{2}.[(pk_decode pk{2}).`2]) *^ r{2} + e1{2})))) = 
-  m_encode m{2} &+ noise_exp (oget RO_H.RO.m{2}.[(pk_decode pk{2}).`2]) (sk_decode sk){2}  e{2} r{2} e1{2}
-                     e2{2} m{2}); last by apply good_decode. 
-  by rewrite noise_exp_val /= matrix_props1 matrix_props2; ring.
+     ((sk_decode sk){1}  `<*>`
+      (m_transpose (oget RO_H.RO.m{2}.[(pk_decode pk{1}).`2]) *^ r{2} + e1{2} +
+       rnd_err_u (m_transpose (oget RO_H.RO.m{2}.[(pk_decode pk{1}).`2]) *^ r{2} + e1{2})))) = 
+  m_encode m{2} &+ noise_exp (oget RO_H.RO.m{2}.[(pk_decode pk{1}).`2]) (sk_decode sk){1}  e{2} r{2} e1{2}
+                     e2{2} m{2});  
+   1: by rewrite noise_exp_val /= matrix_props1 matrix_props2; ring.
+   by smt(good_decode).
 
-seq 9 14 : ((tr{2}, b{2}) = witness /\
+seq 14 9 : ((tr{1}, b{1}) = witness /\
            ={RO_H.RO.m,r,s,e,e1,e2,sd,_A,glob Sim, glob A} /\
-           sd0{2} = sd{1} /\
-           pk{2} = pk_encode (t,sd){2} /\
-           sk{2} = sk_encode s{2} /\
-           t{2} = _A{2} *^ s{2} + e{2} /\
-           sd{2} \in RO_H.RO.m{2} /\
-           oget RO_H.RO.m{2}.[sd{2}] = _A{2}); last first.
-+ exlim _A{2}, sd{2} => _A sd.
-  call(_: ={glob RO_H.RO, glob Sim} /\ oget RO_H.RO.m{2}.[sd] = _A /\ sd \in RO_H.RO.m{2} ). 
-  + proc *;call(_: ={glob RO_H.RO}  /\ oget RO_H.RO.m{2}.[sd] = _A /\ sd \in RO_H.RO.m{2} ).
+           sd0{1} = sd{2} /\
+           pk{1} = pk_encode (t,sd){1} /\
+           sk{1} = sk_encode s{1} /\
+           t{1} = _A{1} *^ s{1} + e{1} /\
+           sd{1} \in RO_H.RO.m{1} /\
+           oget RO_H.RO.m{1}.[sd{1}] = _A{1}); last first.
++ exlim _A{1}, sd{1} => _A sd.
+  call(_: ={glob RO_H.RO, glob Sim} /\ oget RO_H.RO.m{1}.[sd] = _A /\ sd \in RO_H.RO.m{1} ). 
+  + proc *;call(_: ={glob RO_H.RO}  /\ oget RO_H.RO.m{1}.[sd] = _A /\ sd \in RO_H.RO.m{1} ).
     + by proc; auto => />; smt(get_setE).
     by auto => />; smt(get_setE sk_encodeK pk_encodeK).
   by auto => />; smt(sk_encodeK get_setE pk_encodeK).
@@ -830,9 +640,7 @@ lemma parts_work _A s e r e1 e2 m :
   noise_exp _A s e r e1 e2 m =
   noise_exp_part1 s e r e1 e2 &+ (ZR.([-]) (noise_exp_part2 _A s r e1)) &+ noise_exp_part3 _A s e r e2 m by rewrite noise_exp_val /noise_exp_simpl /noise_exp_part1 /noise_exp_part2 /noise_exp_part3 /=; ring. 
 
-module CB(Sim : Simulator_t,A : CAdversaryRO, O : RO_H.RO) = {
-  module H = RO_H.Pub(O)
-
+module CB(Sim : Simulator_t,A : CORR_ADV, O : RO_H.RO) = {
   var s : vector
   var e : vector
   var _A : matrix
@@ -850,15 +658,15 @@ module CB(Sim : Simulator_t,A : CAdversaryRO, O : RO_H.RO) = {
   proc main() = {
     var sd;
     O.init();
-    Sim(H).init();
+    Sim(O).init();
     sd <$ dseed;
-    _A <@ H.h(sd);
+    _A <@ O.get(sd);
     r <$ dshort;
     s <$ dshort;
     e <$ dshort;
     e1 <$ dshort;
     e2 <$ dshort_R;
-    m <@ A(Sim(H)).find(pk_encode (_A *^ s + e,sd),sk_encode s);
+    m <@ A(Sim(O)).find(pk_encode (_A *^ s + e,sd),sk_encode s);
     n1 <- noise_exp_part1 s e r e1 e2;
     n2 <- noise_exp_part2 _A s r e1;
     n3 <- noise_exp_part3 _A s e r e2 m;
@@ -881,12 +689,12 @@ axiom cv_bound_valid _A s e r e2 m :
 
 section.
 
-declare module A <: CAdversaryRO {-LRO,-RO, -RO_H.RO, -CB}.
+declare module A <: CORR_ADV {-LRO,-RO, -RO_H.RO, -CB}.
 declare module S <: Sampler {-A,-LRO,-RO, -RO_H.RO, -CB}.
 declare module Sim <: Simulator_t {-S, -A,-LRO,-RO, -RO_H.RO, -CB}.
 
 lemma correctness_split_aux &m cu_bound cv_bound failprob1 failprob2 failprob3:
-  (forall (O <: RO_SMP.ROpub), islossless O.h => islossless A(O).find) =>
+  (forall (O <: SMP_RO), islossless O.get => islossless A(O).find) =>
   Pr[ CB(Sim,A,RO_H.LRO).main() @ &m : 
         !under_noise_bound CB.n1 (max_noise - cu_bound - cv_bound)] <= failprob1 =>
   Pr[ CB(Sim,A,RO_H.LRO).main() @ &m : 
@@ -930,26 +738,19 @@ module CB1 = {
 }.
 
 lemma cb1 &m cu_bound cv_bound : 
-  (forall (O <: RO_H.ROpub), islossless O.h => islossless Sim(O).init) =>
-  (forall (O <: RO_H.ROpub), islossless O.h => islossless Sim(O).h) =>
-  (forall (O <: RO_SMP.ROpub), islossless O.h => islossless A(O).find) =>
+  (forall (O <: Ideal_RO), islossless O.get => islossless Sim(O).init) =>
+  (forall (O <: Ideal_RO), islossless O.get => islossless Sim(O).get) =>
+  (forall (O <: SMP_RO), islossless O.get => islossless A(O).find) =>
   Pr[ CB(Sim,A,RO_H.LRO).main() @ &m : 
         !under_noise_bound CB.n1 (max_noise - cu_bound - cv_bound)] =
   Pr[ CB1.main(cu_bound,cv_bound) @ &m : res].
 move => S_i_ll S_h_ll A_ll.
 byequiv => //; proc; inline *.
-wp;call{1}(_: true ==> true); 1: by apply (A_ll ( (Sim(RO_H.LROpub))));  apply (S_h_ll (RO_H.LROpub)); apply RO_H.RO_get_ll; smt(duni_matrix_ll). 
+wp;call{1}(_: true ==> true); 1: by apply (A_ll ( (Sim(RO_H.LRO))));  apply (S_h_ll (RO_H.LRO)); apply RO_H.RO_get_ll; smt(duni_matrix_ll). 
 rcondt{1}6; 1: by move => *; auto => />;call(_: true);auto => />;smt(mem_empty).
-auto => />;call {1} (_: true ==> true); 1: by  apply (S_i_ll (RO_H.LROpub)); apply RO_H.RO_get_ll; smt(duni_matrix_ll).  
+auto => />;call {1} (_: true ==> true); 1: by  apply (S_i_ll (RO_H.LRO)); apply RO_H.RO_get_ll; smt(duni_matrix_ll).  
 by auto => />;smt(duni_matrix_ll).
 qed.
-
-(*
-  let u = m_transpose _A *^ r + e1 in
-  let cu = rnd_err_u u in
-    (s `<*>` cu).
-
-*)
 
 module CB2pre = {
   proc main(cu_bound : int) = {
@@ -976,19 +777,19 @@ module CB2 = {
 
 
 lemma cb2pre &m cu_bound: 
-  (forall (O <: RO_H.ROpub), islossless O.h => islossless Sim(O).init) =>
-  (forall (O <: RO_H.ROpub), islossless O.h => islossless Sim(O).h) =>
-  (forall (O <: RO_SMP.ROpub), islossless O.h => islossless A(O).find) =>
+  (forall (O <: Ideal_RO), islossless O.get => islossless Sim(O).init) =>
+  (forall (O <: Ideal_RO), islossless O.get => islossless Sim(O).get) =>
+  (forall (O <: SMP_RO), islossless O.get => islossless A(O).find) =>
   Pr[ CB(Sim,A,RO_H.LRO).main() @ &m : 
         !under_noise_bound CB.n2 cu_bound] =
   Pr[ CB2pre.main(cu_bound) @ &m : res].
 move => S_i_ll S_h_ll A_ll.
 byequiv => //; proc; inline *.
-wp;call{1}(_: true ==> true); 1: by apply (A_ll ( (Sim(RO_H.LROpub))));  apply (S_h_ll (RO_H.LROpub)); apply RO_H.RO_get_ll; smt(duni_matrix_ll). 
+wp;call{1}(_: true ==> true); 1: by apply (A_ll ( (Sim(RO_H.LRO))));  apply (S_h_ll (RO_H.LRO)); apply RO_H.RO_get_ll; smt(duni_matrix_ll). 
 rcondt{1}6; 1: by move => *; auto => />;call(_: true);auto => />; smt(mem_empty).
 rnd{1};rnd;rnd{1}.
 auto => />; 1: by smt(). 
-call {1} (_: true ==> true); 1: by  apply (S_i_ll (RO_H.LROpub)); apply RO_H.RO_get_ll; smt(duni_matrix_ll).  
+call {1} (_: true ==> true); 1: by  apply (S_i_ll (RO_H.LRO)); apply RO_H.RO_get_ll; smt(duni_matrix_ll).  
 by auto => />;smt(dshort_R_ll dshort_ll get_set_sameE).
 qed.
 
@@ -1046,21 +847,19 @@ qed.
 
 *)
 
-module CB3(Sim : Simulator_t,A : CAdversaryRO, O : RO_H.RO) = {
-  module H = RO_H.Pub(O)
-
+module CB3(Sim : Simulator_t,A : CORR_ADV, O : RO_H.RO) = {
   proc main(cv_bound : int) = {
     var sd,_A,r,s,e,e1,e2,m,n;
     O.init();
-    Sim(H).init();
+    Sim(O).init();
     sd <$ dseed;
-    _A <@ H.h(sd);
+    _A <@ O.get(sd);
     r <$ dshort;
     s <$ dshort;
     e <$ dshort;
     e1 <$ dshort;
     e2 <$ dshort_R;
-    m <@ A(Sim(H)).find(pk_encode (_A *^ s + e,sd),sk_encode s);
+    m <@ A(Sim(O)).find(pk_encode (_A *^ s + e,sd),sk_encode s);
     n <- noise_exp_part3 _A s e r e2 m;
     return !under_noise_bound n cv_bound;
   }
@@ -1083,9 +882,9 @@ qed.
 
 lemma correctness_split &m cu_bound cv_bound epsilon failprob1 failprob2 failprob3 :
   (glob Bcb2){m} = cu_bound =>
-  (forall (O <: RO_H.ROpub), islossless O.h => islossless Sim(O).init) =>
-  (forall (O <: RO_H.ROpub), islossless O.h => islossless Sim(O).h) =>
-  (forall (O <: RO_SMP.ROpub), islossless O.h => islossless A(O).find) =>
+  (forall (O <: Ideal_RO), islossless O.get => islossless Sim(O).init) =>
+  (forall (O <: Ideal_RO), islossless O.get => islossless Sim(O).get) =>
+  (forall (O <: SMP_RO), islossless O.get => islossless A(O).find) =>
   (* We need indiff from the nice ROM *)
   (forall trb (D0 <: Distinguisher_t {-S,-LRO,-RO,-RO_H.LRO,-RO_H.RO,  -Sim}),
      `| Pr[ WIndfReal(D0,S,RO_SMP.LRO).main(trb) @ &m : res] - 
@@ -1095,9 +894,9 @@ lemma correctness_split &m cu_bound cv_bound epsilon failprob1 failprob2 failpro
   Pr[ CB2.main(cu_bound) @ &m : res] <= failprob2 =>
   Pr[ CB3(Sim,A,RO_H.LRO).main(cv_bound) @ &m : res] <= failprob3 =>
 
-  Pr[ CorrectnessAdvROM(MLWE_PKE(S(RO_SMP.LROpub)),A,RO_SMP.LRO).main() @ &m : res]  >=
-  1%r - `| Pr[MLWE(Bcb2).main(false) @ &m : res] - Pr[MLWE(Bcb2).main(true) @ &m : res]| 
-      - failprob1 - failprob2 - failprob3 - epsilon.
+  Pr[ Correctness_Adv(RO_SMP.LRO,MLWE_PKE(S(RO_SMP.LRO)),A).main() @ &m : res]  <=
+   `| Pr[MLWE(Bcb2).main(false) @ &m : res] - Pr[MLWE(Bcb2).main(true) @ &m : res]| 
+      + failprob1 + failprob2 + failprob3 + epsilon.
 move => meminit S_i_ll S_h_ll A_ll ind fp1 fp2 fp3.
 have := (correctness A S Sim &m epsilon  S_i_ll S_h_ll A_ll ind).
 rewrite -(cb1 &m cu_bound cv_bound S_i_ll S_h_ll A_ll) in fp1.
@@ -1121,9 +920,9 @@ qed.
 
 lemma correctness_max &m cu_bound epsilon failprob1 failprob2 :
   (glob Bcb2){m} = cu_bound =>
-  (forall (O <: RO_H.ROpub), islossless O.h => islossless Sim(O).init) =>
-  (forall (O <: RO_H.ROpub), islossless O.h => islossless Sim(O).h) =>
-  (forall (O <: RO_SMP.ROpub), islossless O.h => islossless A(O).find) =>
+  (forall (O <: Ideal_RO), islossless O.get => islossless Sim(O).init) =>
+  (forall (O <: Ideal_RO), islossless O.get => islossless Sim(O).get) =>
+  (forall (O <: SMP_RO), islossless O.get => islossless A(O).find) =>
   (* We need indiff from the nice ROM *)
   (forall trb (D0 <: Distinguisher_t {-S,-LRO,-RO,-RO_H.LRO,-RO_H.RO,  -Sim}),
      `| Pr[ WIndfReal(D0,S,RO_SMP.LRO).main(trb) @ &m : res] - 
@@ -1132,9 +931,9 @@ lemma correctness_max &m cu_bound epsilon failprob1 failprob2 :
   Pr[ CB1.main(cu_bound, cv_bound_max) @ &m : res] <= failprob1 =>
   Pr[ CB2.main(cu_bound) @ &m : res] <= failprob2 =>
 
-  Pr[ CorrectnessAdvROM(MLWE_PKE(S(RO_SMP.LROpub)),A,RO_SMP.LRO).main() @ &m : res]  >=
-  1%r - `| Pr[MLWE(Bcb2).main(false) @ &m : res] - Pr[MLWE(Bcb2).main(true) @ &m : res]| 
-      - failprob1 - failprob2  - epsilon.
+  Pr[ Correctness_Adv(RO_SMP.LRO,MLWE_PKE(S(RO_SMP.LRO)),A).main() @ &m : res]  <=
+    `| Pr[MLWE(Bcb2).main(false) @ &m : res] - Pr[MLWE(Bcb2).main(true) @ &m : res]| 
+      + failprob1 + failprob2  + epsilon.
 move => meminit S_i_ll S_h_ll A_ll ind fp1 fp2.
 have := (correctness_split &m cu_bound cv_bound_max epsilon  failprob1 failprob2 0%r meminit S_i_ll S_h_ll A_ll ind fp1 fp2 _).
 + by have := cb3_max &m; smt().
@@ -1163,9 +962,9 @@ import SMP_vs_ROM_IND.
 import MLWE_ROM.
 import MLWE_vs_MLWE_ROM.
 
-module (Sim : Simulator_t) (O : RO_H.ROpub) = {
+module (Sim : Simulator_t) (O : Ideal_RO) = {
   proc init() = {}
-  proc h = S(O).sampleA
+  proc get = S(O).sampleA
 }.
 
 
@@ -1180,16 +979,15 @@ call(_: (glob RO_SMP.RO){1} = (glob RO_H.RO){2}).
 by inline *; auto => />.
 qed.
 
+import PKE_ROM.
 
-import PKE_.
 section.
-
-declare module A <: AdversaryRO {-B1ROM, -B2ROM, -RO_H.LRO,-RO_H.RO, -RO_H.FRO, -RO_SMP.LRO,  -B,-Bt, -BS, -D}.
+declare module A <: Adversary {-B1ROM, -B2ROM, -RO_H.LRO,-RO_H.RO, -RO_H.FRO, -RO_SMP.LRO,  -B,-Bt, -BS, -D}.
 
 lemma main_theorem &m :
-  (forall (O <: RO_SMP.ROpub), islossless O.h => islossless A(O).guess) =>
-  (forall (O <: RO_H.ROpub), islossless O.h => islossless A(O).choose) =>
-  `| Pr[CPAROM(MLWE_PKE(S(RO_SMP.LROpub)),A,RO_SMP.LRO).main() @ &m : res] -  1%r / 2%r | <=
+  (forall (O <: SMP_RO), islossless O.get => islossless A(O).guess) =>
+  (forall (O <: Ideal_RO), islossless O.get => islossless A(O).choose) =>
+  `| Pr[CPA(RO_SMP.LRO,MLWE_PKE(S(RO_SMP.LRO)),A).main() @ &m : res] -  1%r / 2%r | <=
     `| Pr[MLWE(B(BS(B1ROM(A,S),Sim),RO_H.LRO)).main(false) @ &m : res] -
        Pr[MLWE(B(BS(B1ROM(A,S),Sim),RO_H.LRO)).main(true) @ &m : res] | + 
     `| Pr[MLWE(Bt(BS(B2ROM(A,S),Sim),RO_H.LRO)).main(false) @ &m : res]-
@@ -1209,20 +1007,20 @@ end section.
 
 section.
 
-declare module A <: CAdversaryRO {-RO_H.LRO,-RO_H.RO, -RO_H.FRO, -RO_SMP.LRO, -CB}.
+declare module A <: CORR_ADV {-RO_H.LRO,-RO_H.RO, -RO_H.FRO, -RO_SMP.LRO, -CB}.
 
 lemma correctness_max &m cu_bound failprob1 failprob2 :
   (glob Bcb2){m} = cu_bound =>
-  (forall (O <: RO_H.ROpub), islossless O.h => islossless Sim(O).init) =>
-  (forall (O <: RO_H.ROpub), islossless O.h => islossless Sim(O).h) =>
-  (forall (O <: RO_SMP.ROpub), islossless O.h => islossless A(O).find) =>
+  (forall (O <: Ideal_RO), islossless O.get => islossless Sim(O).init) =>
+  (forall (O <: Ideal_RO), islossless O.get => islossless Sim(O).get) =>
+  (forall (O <: SMP_RO), islossless O.get => islossless A(O).find) =>
 
   Pr[ CB1.main(cu_bound, cv_bound_max) @ &m : res] <= failprob1 =>
   Pr[ CB2.main(cu_bound) @ &m : res] <= failprob2 =>
 
-  Pr[ CorrectnessAdvROM(MLWE_PKE(S(RO_SMP.LROpub)),A,RO_SMP.LRO).main() @ &m : res]  >=
-  1%r - `| Pr[MLWE(Bcb2).main(false) @ &m : res] - Pr[MLWE(Bcb2).main(true) @ &m : res]| 
-      - failprob1 - failprob2.
+  Pr[ Correctness_Adv(RO_SMP.LRO,MLWE_PKE(S(RO_SMP.LRO)),A).main() @ &m : res]  <=
+    `| Pr[MLWE(Bcb2).main(false) @ &m : res] - Pr[MLWE(Bcb2).main(true) @ &m : res]| 
+      + failprob1 + failprob2.
 move => cb2_val S_i_ll S_h_ll A_ll fp1 fp2.
 have := (correctness_max A S Sim &m cu_bound 0%r failprob1 failprob2 cb2_val S_i_ll S_h_ll A_ll _ fp1 fp2 ).
 move => trb D0; have -> : trb = (trb.`1,trb.`2) by smt().
